DeBruijnSSA/BinSyntax/Rewrite/Region/Structural.lean
@@ -119,15 +119,27 @@ theorem Eqv.packed_case {Γ : Ctx α ε} {R : LCtx α}
     (let1 (pair (var 1 (by simp)) (var 0 Ctx.Var.shead)) s.packed) := by
   simp only [packed, packed_out_case, packed_in_case]
 
-theorem Eqv.packed_cfg {Γ : Ctx α ε} {L R : LCtx α} {β : Eqv φ Γ (R ++ L)} {G}
+theorem Eqv.packed_cfg_unpack {Γ : Ctx α ε} {L R : LCtx α} {β : Eqv φ Γ (R ++ L)} {G}
   : (cfg R β G).packed (Δ := Δ)
-  = gloop R.pack β.packed.unpacked_app_out
+  = gloop R.pack
+      β.packed.unpacked_app_out
       (unpack.lsubst (Subst.Eqv.fromFCFG (λi =>
         (let1 (pair (var 2 (by simp)) (var 0 Ctx.Var.shead)) (G i).packed.unpacked_app_out)))) := by
-  rw [packed_def', packed_in_cfg, packed_out_cfg_gloop, <-packed_def']
+  rw [packed_def', packed_in_cfg, packed_out_cfg_gloop_unpack, <-packed_def']
   congr; funext i
   rw [vwk1_unpacked_app_out, packed_out_let1, <-packed_def', <-unpacked_app_out_let1]
   simp
+
+theorem Eqv.packed_cfg {Γ : Ctx α ε} {L R : LCtx α} {β : Eqv φ Γ (R ++ L)} {G}
+  : (cfg R β G).packed (Δ := Δ)
+  = gloop R.pack
+      β.packed.unpacked_app_out
+      (pack_coprod
+        (λi => (let1 (pair (var 1 (by simp)) (var 0 Ctx.Var.shead)) (G i).packed.unpacked_app_out)))
+  := by
+  rw [packed_def', packed_in_cfg, packed_out_cfg_gloop, <-packed_def']
+  congr; funext i
+  rw [packed_out_let1, <-packed_def', unpacked_app_out_let1]
 
 end Region
 
